Add example for demo.

LeanCats/Examples.lean
@@ -2,7 +2,6 @@ import LeanCats.Data
 import LeanCats.Relations
 import LeanCats.Theoriems
 import LeanCats.Basic
-import LeanCats.Macro
 
 open CatRel
 open Data
@@ -14,10 +13,10 @@ variable (coConst : IsStrictTotalOrder Event (preCo evts))
 @[simp] def X : CandidateExecution :=
   {
     evts := evts
-    po := CatRel.po evts
-    fr := CatRel.fr evts
-    rf := CatRel.rf.wellformed evts
-    IW := evts.IW
+    _po := CatRel.po evts
+    _fr := CatRel.fr evts
+    _rf := CatRel.rf.wellformed evts
+    _IW := evts.IW
   }
 
 /-! ### SC (Sequential Consistency) model reperesentation in Lean 4.
@@ -27,10 +26,10 @@ and the operations of each individual thread appear in this sequence in the orde
 specified by its program.-/
 
 -- We define the communication between threads as com:
-@[simp] def com := (X evts coConst).rf ∪ ((co.wellformed evts) ∪ (X evts coConst).fr)
+@[simp] def com := (X evts coConst)._rf ∪ ((co.wellformed evts) ∪ (X evts coConst)._fr)
 
 -- Then we union it with the po, the SC ensures that every instructions are executed in program order.
-@[simp] def sc := (com evts coConst) ∪ ((X evts coConst).po)
+@[simp] def sc := (com evts coConst) ∪ ((X evts coConst)._po)
 
 -- We should avoid the cyclic, because the fr in a ghb will leads a overwritten that violates the program order.
 @[simp] def assert := Acyclic (sc evts coConst)
@@ -44,20 +43,20 @@ variable (coConst : IsStrictTotalOrder Event (preCo evts))
 @[simp] def X : CandidateExecution :=
   {
     evts := evts
-    po := CatRel.po evts
-    fr := CatRel.fr evts
-    rf := CatRel.rf.wellformed evts
-    IW := evts.IW
+    _po := CatRel.po evts
+    _fr := CatRel.fr evts
+    _rf := CatRel.rf.wellformed evts
+    _IW := evts.IW
   }
 
 /-! ### SC (Sequential Consistency) model reperesentation in Lean 4.
 A TSO is a memory model that allows the write read out of order in the same thread (write buffer).-/
 
 -- We define the communication between threads as com as in SC:
-@[simp] def com := (external evts ∩ (X evts coConst).rf) ∪ (co.wellformed evts ∪ ((X evts coConst).fr))
+@[simp] def com := (external evts ∩ (X evts coConst)._rf) ∪ (co.wellformed evts ∪ ((X evts coConst)._fr))
 
 -- Then we minus the internal read from and W*R from the po, because we allow them to be out of order.
-@[simp] def po_tso := (X evts coConst).po ∩ ((prod W W) ∪ (prod R M))
+@[simp] def po_tso := (X evts coConst)._po ∩ ((prod W W) ∪ (prod R M))
 
 @[simp] def ghb := (po_tso evts coConst) ∪ (com evts coConst)
 
@@ -69,6 +68,8 @@ end TSO01
 -- The set of accepted candidate executions of SC is the subset of the TSO, because SC rejected more than TSO.
 -- Which means sc imples tso, the sc is stronger.
 -- In this case, if we find the ghb is acyclic then tso must also be acyclic because sc models more edges.
+
+#check SC.assert
 
 -- https://leanprover-community.github.io/mathlib4_docs/Mathlib/Order/Defs/Unbundled.html#IsIrrefl
 theorem scvtso
@@ -103,10 +104,3 @@ by
       exact h
     }
   }
-
--- Automated loading of memory model.
--- Let's define the sc in the cat langague model instead of writing it explicitly.
-section Example1
-open CatGrammar
-
-end Example1
