LeanCats/tsoWeakerThanSc.lean
@@ -1,20 +1,63 @@
 import LeanCats.Macro
+import LeanCats.Reader
+import LeanCats.Data
+import LeanCats.Relations
+import LeanCats.Theoriems
+import LeanCats.Basic
 
--- include "cos.cat"
-[model| sc
-  let com = rf | co | fr
-  let poo = po & (W*W | R*M)
+-- -- include "cos.cat"
+-- [model| sc
+--   let com = rf | co | fr
+--   let poo = po & (W*W | R*M)
+--
+--   let ghb = po | com
+--   acyclic ghb as new
+-- ]
+--
+-- [model| tso
+--   let com_tso = rf | co | fr
+--   let po_tso = po & (W*W | R*M)
+--   let ghb = po_tso | com_tso
+--   acyclic ghb as new
+-- ]
+--
+-- #check sc.new
+-- #check tso.new
 
-  let ghb = po | com
-  acyclic ghb as new
-]
+defcat <"tso.cat">
+defcat <"sc.cat">
 
-[model| tso
-  let com_tso = rf | co | fr
-  let po_tso = po & (W*W | R*M)
-  let ghb = po_tso | com_tso
-  acyclic ghb as new
-]
-
-#check sc.new
-#check tso.new
+theorem scvtso
+  (evts : Data.Events)
+  [IsStrictTotalOrder Data.Event (CatRel.preCo evts)]
+  (X : CandidateExecution evts)
+  : sc.sc evts X → tso.tso evts X :=
+by
+  unfold sc.sc
+  simp
+  intro sc
+  apply ayclicMono sc
+  intro a b
+  intro tso
+  cases tso with
+  | inl h => {
+    simp at h
+    apply Or.inr
+    obtain ⟨l, r⟩ := h
+    exact l
+  }
+  | inr h => {
+    obtain ⟨l⟩ := h
+    {
+      apply Or.inl
+      apply Or.inl
+      obtain ⟨l, r⟩ := l
+      exact r
+    }
+    {
+      rename_i h
+      apply Or.inl
+      apply Or.inr
+      exact h
+    }
+  }
